\begin{align*}
K_{clm} &\sim \operatorname{N}(e^{\alpha_{c}}(K_{l}^o+\delta_{l}\gamma_{cl}),(e^{ \tau_{cl}^K })^{-1})\\
\gamma_{cl}&=\begin{cases}
0  & \text{if } c=0;\\
\operatorname{N}(0,{(e^{\sigma^{\gamma}})}^{-1}) & \text{if } c=1.
\end{cases}\\
\\
\pi(\gamma_{2l}|\theta)&=\sqrt{\frac{e^{\sigma^{\gamma}}}{2\pi}} e^{-\frac{1}{2}(\gamma_{cl})^{2}e^{\sigma^{\gamma}} }
\prod_{m=1}{M_{2l}}
\sqrt{\frac{e^{ \tau_{2l}^K }}{2\pi}} e^{-\frac{1}{2}(K_{2lm}-e^{\alpha_{2}}(K_{l}^o+\delta_{l}\gamma_{2l}))^{2} e^{ \tau_{2l}^K }}\\
\text{Taking logs}\\
\color{red}{l\pi(\gamma_{2l}|\theta)}&
\color{red}{
=-\frac{1}{2}(\gamma_{2l})^{2}e^{\sigma^{\gamma}}
-
\sum_{m=1}^{M_{2l}}\frac{1}{2}(K_{2lm}-e^{\alpha_{2}}(K_{l}^o+\delta_{l}\gamma_{2l}))^{2}e^{\tau_{2l}^K}
+C
}\\
\text{Similarly for $\omega_{2l}$}\\
\color{red}{l\pi(\omega_{2l}|\theta)}&
\color{red}{
=-\frac{1}{2}(\omega_{2l})^{2}e^{\sigma^{\omega}}
-
\sum_{m=1}^{M_{2l}}\frac{1}{2}(r_{2lm}-e^{\beta_{2}}(r_{l}^o+\delta_{l}\omega_{2l}))^{2}e^{\tau_{2l}^r}
+C
}
\end{align*}

\begin{center}
\line(1,0){250}
\end{center}

\begin{align*}
\text{$\sigma^{\gamma}$ is similar to both $\sigma^{K,o}$ and $\sigma^{r,o}$}\\
\color{red}{l\pi(\sigma^{\gamma}|\theta)}&
\color{red}{
=-\frac{1}{2}(\sigma^{\gamma}-\eta^{\gamma})^{2}\psi^{\gamma} 
+
\sum_{m=1}^{M_{2l}}\frac{1}{2}(\sigma^{\gamma}-(\gamma_{2l})^{2}e^{\sigma^{\gamma}})
+C
}\\
\\
\text{$\sigma^{\omega}$ is similar to both $\sigma^{K,o}$ and $\sigma^{r,o}$}\\
\color{red}{l\pi(\sigma^{\omega}|\theta)}&
\color{red}{
=-\frac{1}{2}(\sigma^{\omega}-\eta^{\omega})^{2}\psi^{\omega} 
+
\sum_{m=1}^{M_{2l}}\frac{1}{2}(\sigma^{\omega}-(\omega_{2l})^{2}e^{\sigma^{\omega}})
+C
}
\end{align*}

\begin{center}
\line(1,0){250}
\end{center}

\begin{align*}
K_{clm} &\sim \operatorname{N}(e^{\alpha_{c}}(K_{l}^o+\delta_{l}\gamma_{cl}),(e^{ \tau_{cl}^K })^{-1})\\
\alpha_{c}&=\begin{cases}
1  & \text{if } c=0;\\
\operatorname{N}(\alpha^{\mu},\eta^{\alpha})  & \text{if } c=1.
\end{cases}\\
\\
\pi(\alpha_{2}|\theta)&=
\sqrt{\frac{\eta^{\alpha}}{2\pi}} e^{-\frac{1}{2}(\alpha_{2}-\alpha^{\mu})^{2}\eta^{\alpha} }
\prod_{m=1}{M_{2l}}
\sqrt{\frac{e^{ \tau_{2l}^K }}{2\pi}} e^{-\frac{1}{2}(K_{2lm}-e^{\alpha_{2}}(K_{l}^o+\delta_{l}\gamma_{2l}))^{2}e^{ \tau_{2l}^K } }\\
\text{Taking logs}\\
\color{red}{l\pi(\alpha_{2}|\theta)}&
\color{red}{
=-\frac{1}{2}(\alpha_{2}-\alpha^{\mu})^{2}\eta^{\alpha}  
+
\sum_{m=1}^{M_{2l}}\frac{1}{2}(K_{2lm}-e^{\alpha_{2}}(K_{l}^o+\delta_{l}\gamma_{2l}))^{2}e^{\sigma^{\tau_{2l}^K}}
+C
}\\
\text{Similarly for $\beta_{2}$}\\
\color{red}{l\pi(\beta_{2}|\theta)}&
\color{red}{
=-\frac{1}{2}(\beta_{2}-\beta^{\mu})^{2}\eta^{\beta}  
+
\sum_{m=1}^{M_{2l}}\frac{1}{2}(r_{2lm}-e^{\beta_{2}}(r_{l}^o+\delta_{l}\omega_{2l}))^{2}e^{\sigma^{\tau_{2l}^r}}
+C
}
\end{align*}


\begin{center}
\line(1,0){250}
\end{center}


\begin{align*}
y_{clmn} &\sim \operatorname{N}(\hat{y}_{clmn},(e^{ \upsilon_{l}+\nu_{c}  })^{-1} ) \\
\upsilon_{c} &\sim \operatorname{N}(\upsilon^{\mu},(e^{ \sigma^{\upsilon} })^{-1})\\
\\
\pi(\upsilon_{2}|\theta)&=\sqrt{\frac{e^{ \sigma^{\upsilon} }}{2\pi}} e^{-\frac{1}{2}(\upsilon_{2}-\upsilon_{\mu})^{2}e^{ \sigma^{\upsilon} } }
\prod_{l=1}^{L}\prod_{m=1}^{M_{2l}}\sqrt{\frac{e^{ \upsilon_{2} }}{2\pi}} e^{-\frac{1}{2}(y_{clmn}-\hat{y}_{clmn})^{2}e^{ \nu_{l} +\upsilon_{2} } }\\
\text{Taking logs}\\
\color{red}{l\pi(\upsilon_{2}|\theta)}&
\color{red}{
=-\frac{1}{2}(\upsilon_{2}-\upsilon^{\mu})^{2}e^{ \sigma^{\upsilon} } 
+
\sum_{l=1}^{L}\sum_{m=1}^{M_{2l}}\frac{1}{2}(\upsilon_{c}-(y_{clmn}-\hat{y}_{clmn})^{2}e^{\nu_{l}+\upsilon_{c} })
+C}
\end{align*}

\begin{align*}
\text{$\sigma^{\upsilon}$ is similar to both $\sigma^{Z}$ and $\sigma^{\nu}$}\\
\color{red}{l\pi(\sigma^{\upsilon}|\theta)}
\color{red}{
=-\frac{1}{2}(\sigma^{\upsilon}-\eta^{\upsilon})^{2}\psi^{\upsilon}
+
\frac{1}{2}(\sigma^{\upsilon} -(\upsilon_{2}-\upsilon^{\mu})^{2}e^{\sigma^{\upsilon}})
+C}
\end{align*}
