\begin{align*}
K_{clm} &\sim \operatorname{N}(e^{\alpha_{c}+(K_{l}^o+\delta_{l}\gamma_{cl})},(e^{ \tau_{cl}^K })^{-1})\\
K_{l}^o &\sim \operatorname{N}(K^p, (e^{ \sigma^{K,o} })^{-1} )\\
\\
\pi(K_{l}^o |\theta)&=\sqrt{\frac{e^{ \sigma^{K,o} }}{2\pi}} e^{-\frac{1}{2}(K_{l}^o-K^p)^{2}e^{ \sigma^{K,o} } }
\prod_{c=1}^{2}\prod_{m=1}^{M^{cl}}\sqrt{\frac{e^{ \tau_{cl}^K }}{2\pi}} e^{-\frac{1}{2}(K_{clm}-e^{\alpha_{c}+(K_{l}^o+\delta_{l}\gamma_{cl})})^{2}e^{ \tau_{cl}^K } }\\
\text{Taking logs}\\
\color{red}{l\pi(K_{l}^o |\theta)}&
\color{red}{
=-\frac{1}{2}(K_{l}^o-K^p)^{2}e^{ \sigma^{K,o} } 
+
\sum_{c=1}^{2}\sum_{m=1}^{M^{cl}}\frac{1}{2}(K_{clm}-e^{\alpha_{c}+(K_{l}^o+\delta_{l}\gamma_{cl})^{2}}e^{\tau_{cl}^K}
+C}\\
\text{Similarly for $r_{l}^o$}\\
\color{red}{l\pi(r_{l}^o |\theta)}&
\color{red}{
=-\frac{1}{2}(r_{l}^o-r^p)^{2}e^{ \sigma^{r,o} } 
+
\sum_{c=1}^{2}\sum_{m=1}^{M^{cl}}\frac{1}{2}(r_{clm}-e^{\beta_{c}+(r_{l}^o+\delta_{l}\omega_{cl})^{2}}e^{\tau_{cl}^r}
+C}
\end{align*}

\begin{center}
\line(1,0){250}
\end{center}

\begin{align*}
y_{clmn} &\sim \operatorname{N}(\hat{y}_{clmn},(e^{ \upsilon_{l}+\nu_{c}  })^{-1} ) \\
\nu_{l} &\sim \operatorname{N}(\nu_{\mu},(e^{ \sigma^{\nu} })^{-1})\\
\\
\pi(\nu_{l}|\theta)&=\sqrt{\frac{e^{ \sigma^{\nu} }}{2\pi}} e^{-\frac{1}{2}(\nu_{l}-\nu_{\mu})^{2}e^{ \sigma^{\nu} } }
\prod_{c=1}^{2}\prod_{m=1}^{M_{cl}}\sqrt{\frac{e^{ \nu_{l}+\upsilon{c} }}{2\pi}} e^{-\frac{1}{2}(y_{clmn}-\hat{y}_{clmn})^{2}e^{ \nu_{l}+\upsilon{c} } }\\
\text{Taking logs}\\
\color{red}{l\pi(\nu_{l}|\theta)}&
\color{red}{
=-\frac{1}{2}(\nu_{l}-\nu_{\mu})^{2}e^{ \sigma^{\nu} } 
+
\sum_{c=1}^{2}\sum_{m=1}^{M_{cl}}\frac{1}{2}(\nu_{l}-(y_{clmn}-\hat{y}_{clmn})^{2}e^{ \nu_{l} +\upsilon_{c} })
+C}
\end{align*}

\begin{center}
\line(1,0){250}
\end{center}

\begin{align*}
K_{clm} &\sim \operatorname{N}(e^{\alpha_{c}+(K_{l}^o+\delta_{l}\gamma_{cl})},(e^{ \tau_{cl}^K })^{-1})\\
r_{clm} &\sim \operatorname{N}(e^{\beta_{c}+(r_{l}^o+\delta_{l}\omega_{cl})},(e^{ \tau_{cl}^r })^{-1})\\
\delta_{l} &\sim Bern(p)\\
\color{red}{
\pi(y_{2lm}|,\delta_{l}=1,\theta)}&
\color{red}{
=(p)\times
\prod_{m=1}^{m_{2l}}
\sqrt{\frac{e^{ \tau_{2l}^K }}{2\pi}} e^{-\frac{1}{2}(K_{2lm}-e^{\alpha_{c}+(K_{l}^o+\delta_{l}\gamma_{2l})})^{2}e^{ \tau_{2l}^K } }
\sqrt{\frac{e^{ \tau_{2l}^r }}{2\pi}} e^{-\frac{1}{2}(r_{2lm}-e^{\beta_{c}+(r_{l}^o+\delta_{l}\omega_{2l})})^{2}e^{ \tau_{2l}^r } }
}
\\
\color{red}{
\pi(y_{2lm}|,\delta_{l}=0,\theta)}&
\color{red}{
=(1-p)\times
\prod_{m=1}^{m_{2l}}
\sqrt{\frac{e^{ \tau_{2l}^K }}{2\pi}} e^{-\frac{1}{2}(K_{2lm}-e^{\alpha_{2}+(K_{l}^o)})^{2}e^{ \tau_{2l}^K } }
\sqrt{\frac{e^{ \tau_{2l}^r }}{2\pi}} e^{-\frac{1}{2}(r_{2lm}-e^{\beta_{2}+(r_{l}^o)})^{2}e^{ \tau_{2l}^r } }
}
\end{align*}

\begin{center}
\line(1,0){250}
\end{center}

\begin{align*}
K_{l}^o &\sim \operatorname{N}(K^p, (e^{ \sigma^{K,o} })^{-1} )\\
\sigma^{K,o} &\sim \operatorname{N}(\eta^{K,o}, (\psi^{K,o})^{-1} )\\
\pi(\sigma^{K,o} |\theta)&=
\sqrt{\frac{\psi^{K,o}}{2\pi}} e^{-\frac{1}{2}(\sigma^{K,o}-\eta^{K,o})^{2}\psi^{K,o} }
\prod_{l=1}^{L}
\sqrt{\frac{
e^{ \sigma^{K,o}}
}{2\pi}} e^{-\frac{1}{2}(
K_{l}^o-K^p
)^{2} 
e^{ \sigma^{K,o}}
}\\
\text{Taking logs}\\
\color{red}{l\pi(\sigma^{K,o}|\theta)}&
\color{red}{
=-\frac{1}{2}(\sigma^{K,o}-\eta^{K,o})^{2}\psi^{K,o} 
+
\sum_{l=1}^{L}\frac{1}{2}(\sigma^{K,o}-(K_{l}^o-K^p)^{2}e^{\sigma^{K,o}})
+C
}
\\
\text{Similarly for $\sigma^{r,o}$}\\
\color{red}{l\pi(\sigma^{r,o}|\theta)}&
\color{red}{
=-\frac{1}{2}(\sigma^{r,o}-\eta^{r,o})^{2}\psi^{r,o} 
+
\sum_{l=1}^{L}\frac{1}{2}(\sigma^{r,o}-(r_{l}^o-r^p)^{2}e^{\sigma^{r,o}})
+C
}
\\
\text{and similarly for $\sigma^{\nu}$}\\
\color{red}{l\pi(\sigma^{\nu}|\theta)}&
\color{red}{
=-\frac{1}{2}(\sigma^{\nu}-\eta^{\nu})^{2}\psi^{\nu} 
+
\sum_{l=1}^{L}\frac{1}{2}(\sigma^{\nu}-(\nu_{l}-\nu^p)^{2}e^{\sigma^{\nu}})
+C
}
\end{align*}