\documentclass[11pt,a4paper]{article}
\topmargin=-0.5in
\oddsidemargin=0in
\evensidemargin=0in
\textwidth=6.5in
\textheight=9.5in
\renewcommand{\thefootnote}{\fnsymbol{footnote}}
\usepackage{times,natbib}
\usepackage{amsmath,amsfonts,graphicx}
\usepackage{color}

\begin{document}

\begin{align*}
c&=1,2 \qquad & \text{(Condition)}\\
l&=1,...,L_{c}  \qquad & \text{(ORF)}\\
m&=1,...,M_{cl}      \qquad & \text{(Repeat)}\\
n&=1,...,N_{clm}     \qquad & \text{(Time Point)}\\
\\
y_{clmn} &\sim \operatorname{N}(\hat{y}_{clmn},(e^{ \upsilon_{l}+\nu_{c}  })^{-1} ) \\
\hat{y}_{clmn} &= f(x_{clmn};e^{ K_{clm} } ,e^{ r_{clm} } , e^{ P })\\
\end{align*}

\begin{align*}
K_{clm} &\sim \operatorname{N}(e^{\alpha_{c}+(K_{l}^o+\delta_{l}\gamma_{cl})},(e^{ \tau_{cl}^K })^{-1})\qquad &\tau_{cl}^K &\sim \operatorname{N}(\sigma^{K}, (\phi^{K})^{-1} )\\
r_{clm} &\sim \operatorname{N}(e^{\beta_{c}+(r_{l}^o+\delta_{l}\omega_{cl})},(e^{ \tau_{cl}^r })^{-1})\qquad &\tau_{cl}^r &\sim \operatorname{N}(\sigma^{r}, (\phi^{r})^{-1} )\\
\\
K_{l}^o &\sim \operatorname{N}(K^p, (e^{ \sigma^{K,o} })^{-1} )\qquad &\sigma^{K,o} &\sim \operatorname{N}(\eta^{K,o}, (\psi^{K,o})^{-1} )\\
r_{l}^o &\sim \operatorname{N}(r^p, (e^{ \sigma^{r,o} })^{-1} )\qquad &\sigma^{r,o} &\sim \operatorname{N}(\eta^{r,o}, (\psi^{r,o})^{-1} )\\
\nu_{l} &\sim \operatorname{N}(\nu_{p},(e^{ \sigma^{\nu} })^{-1})\qquad&\sigma^{\nu} &\sim \operatorname{N}(\eta^{\nu}, (\psi^{\nu})^{-1} )\\
\delta_{l} &\sim Bern(p)\\
\\
\gamma_{cl}&= \begin{cases}
0  & \text{if } c=0;\\
\operatorname{N}(0,{(e^{\sigma^{\gamma}})}^{-1}) & \text{if } c=1.
\end{cases}
\qquad
&\sigma^{\gamma}&\sim \operatorname{N}(\eta^{\gamma},\psi^{\gamma})
\\
\omega_{cl}&= \begin{cases}
0  & \text{if } c=0;\\
\operatorname{N}(0,({e^{\sigma^{\omega}})}^{-1}) & \text{if } c=1.
\end{cases}
\qquad
&\sigma^{\omega}&\sim \operatorname{N}(\eta^{\omega},\psi^{\omega})
\end{align*}


\begin{align*}
\alpha_{c}&=\begin{cases}
0  & \text{if } c=0;\\
\operatorname{N}(\alpha^{\mu},\eta^{\alpha})  & \text{if } c=1.
\end{cases}
\\
\beta_{c}&=\begin{cases}
0  & \text{if } c=0;\\
\operatorname{N}(\beta^{\mu},\eta^{\beta}) & \text{if } c=1.
\end{cases}
\\
\upsilon_{c}&=\begin{cases}
0  & \text{if } c=0;\\
\operatorname{N}(\upsilon^{\mu},({e^{\sigma^{\upsilon}}})^{-1}) & \text{if } c=1.
\end{cases}
&\sigma^{\upsilon} &\sim \operatorname{N}(\eta^{\upsilon}, (\psi^{\upsilon})^{-1} )\\
\end{align*}

\begin{align*}
K^p &\sim \operatorname{N}(K^\mu, ({\eta^{K,p}})^{-1} )\\
r^p &\sim \operatorname{N}(r^\mu, ({\eta^{r,p}})^{-1} )\\
\nu^p &\sim \operatorname{N}(\nu^\mu, ({\eta}^{\nu,p})^{-1} )\\
P &\sim \operatorname{N}(P^\mu, ({\eta^{P}})^{-1} )\\
\end{align*}

\newpage

\include{Kclm_rclm}
\include{K_l_r_l}
\include{cl}
\include{K_p_r_p}
\end{document}


\sqrt{\frac{}{2\pi}} e^{-\frac{1}{2}()^{2} }

\prod_{l=1}^{L}\prod_{m=1}^{m_{l}}\prod_{n=1}^{n_{lm}}

\sum_{l=1}^{L}\sum_{m=1}^{M_{l}}\sum_{n=1}^{N_{lm}}

