\documentclass[11pt,a4paper]{article}
\topmargin=-0.5in
\oddsidemargin=0in
\evensidemargin=0in
\textwidth=6.5in
\textheight=9.5in
\renewcommand{\thefootnote}{\fnsymbol{footnote}}
\usepackage{times,natbib}
\usepackage{amsmath,amsfonts,graphicx}
\usepackage{color}

\begin{document}



\begin{align*}
l(K_l,K_{lm})=\prod_{m}^{M_{l}}\operatorname{N}(K_l;K_{lm},\frac{1}{e^{\tau_{K}}})=
\operatorname{N}(K_l;\mu^{*}_{K_l},{\sigma^{*2}_{K_l}})
\end{align*}
\begin{align*}
\mu^{*}_{K_l}=\sum_{m}^{M_{l}} \frac{y_{lm} }{ M_l}
\qquad 
{\sigma^{*2}_{K_l}}=\frac{1 }{ M_{l}e^{\tau_{K}} }
\end{align*}
\begin{align*}
l(K,K_{l})=\prod_{l}^{L}\operatorname{N}(K;\mu^{*}_{K_l},\frac{1}{\frac{1}{e^{\sigma^{*2}_{K_l}}}+{\sigma^{*2}_{K_l}}})=
\operatorname{N}(K;\mu^{*}_{K},{\sigma^{*2}_{K_l}})
\end{align*}

\begin{align*}
\left.\mu^{*}_{K}=\sum_{L}^{l}\frac{\mu^{*}_{K_l}}{\frac{1}{e^{{\sigma^{o2}_{K}}}}+{\sigma^{*2}_{K}}} \middle/ \sum_{L}^{l}\frac{1}{\frac{1}{e^{{\sigma^{o2}_{K}}}}+{\sigma^{*2}_{K}}}  \right.
\qquad 
\left.{\sigma^{*2}_{K_{l}}}=1\middle/
\sum_{L}^{l}\frac{1}{\frac{1}{e^{{\sigma^{o2}_{K}}}}+{\sigma^{*2}_{K}}}\right.
\end{align*}
\begin{align*}
\pi(K|K_{lm})=\operatorname{N}(K;\frac{{\sigma^{*2}_{K}} K_{\mu}+\frac{1}{\eta^{p}_{K}}\mu^{*}_K}{{\sigma^{*2}_{K}}+\frac{1}{\eta^{p}_{K}}},\frac{{\sigma^{*2}_{K}} \frac{1}{\eta^{p}_{K}}}{{\sigma^{*2}_{K}}+\frac{1}{\eta^{p}_{K}}} )
\end{align*}
\begin{align*}
\pi(K_{l}|K,K_{lm})=\operatorname{N}(K_l;
\frac{
	{\sigma^{*2}_{K_{l}}} K + \frac{1}{ e^{ {\sigma^{o2}_{K}} } } \mu^{*}_{K_{l}}
	}{
	{\sigma^{*2}_{K_{l}}} + \frac{1}{ e^{ {\sigma^{o2}_{K}} } }
	}
,\frac{
	{\sigma^{*2}_{K_{l}}} \frac{1}{e^{{\sigma^{o2}_{K}}}}
	}{
	{\sigma^{*2}_{K_{l}}}+\frac{1}{e^{{\sigma^{o2}_{K}}}}} )
\end{align*}

\end{document}
