\begin{align*}
Z_{l} &\sim \operatorname{N}(Z^{p},{(e^{\sigma^{Z}})}^{-1})\\
Z^{p} &\sim N(Z^{\mu},{(\eta^{Z,p})}^{-1}) \\
\pi(Z^{p}|\theta)&=\sqrt{\frac{\eta^{Z,p}}{2\pi}} e^{-\frac{1}{2}(Z^{p}-Z^{\mu})^{2}\eta^{Z,p} }
\prod_{l=1}^{L}\sqrt{\frac{e^{\sigma^{Z}}}{2\pi}} e^{-\frac{1}{2}(Z_{l}-Z^{p})^{2}e^{\sigma^{Z}} }\\
\text{Taking logs}\\
\color{red}{l\pi(Z^{p}|\theta)}&
\color{red}{
=-\frac{1}{2}(Z^{p}-Z^{\mu})^{2}e^{\sigma^{Z}}
-
\sum_{l=1}^{L}\frac{1}{2}(Z_{l}-Z^{p})^{2}e^{\sigma^{Z}}
+C
}\\
\text{Similarly for $\nu^p$}\\
\color{red}{l\pi(\nu^p|\theta)}&
\color{red}{
=-\frac{1}{2}(\nu^{p}-\nu^{\mu})^{2}e^{\sigma^{\nu}}
-
\sum_{l=1}^{L}\frac{1}{2}(\nu_{l}-\nu^{p})^{2}e^{\sigma^{\nu}}
+C
}\\
\text{And also similarly for $\upsilon^p$}\\
\color{red}{l\pi(\upsilon^p|\theta)}&
\color{red}{
=-\frac{1}{2}(\upsilon^{p}-\upsilon^{\mu})^{2}e^{\sigma^{\upsilon}}
-
\sum_{l=1}^{L}\frac{1}{2}(\upsilon_{l}-\upsilon^{p})^{2}e^{\sigma^{\upsilon}}
+C
}
\end{align*}