\begin{align*}
K_{lm} &\sim \operatorname{N}(K_{l}^o, (e^{ \tau_{l}^K })^{-1} )\\
K_{l}^o &\sim \operatorname{N}(K^p, (e^{ \sigma^{K,o} })^{-1} )\\
\\
\pi(K_{l}|\theta)&=
\sqrt{\frac{e^{ \sigma^{K,o} }}{2\pi}} e^{-\frac{1}{2}(K_{l}^o-K^p)^{2}e^{ \sigma^{K,o} } }
\prod_{m=1}^{M_{l}}\sqrt{\frac{e^{ \tau_{l}^K }}{2\pi}} e^{-\frac{1}{2}(K_{lm}-K_{l}^o)^{2}e^{ \tau_{l}^K } }\\
\text{Taking logs}\\
\color{red}{l\pi(K_{l}|\theta)}&
\color{red}{
=-\frac{1}{2}(K_{l}^o-K^p)^{2}e^{\sigma^{K,o} }
-
\sum_{m=1}^{M_{l}}\frac{1}{2}(K_{lm}-K_{l}^o)^{2}e^{ \tau_{l}^K }
+C
}\\
\text{Similarly for $r_{lm}$}\\
\color{red}{l\pi(r_{l}|\theta)}&
\color{red}{
=-\frac{1}{2}(r_{l}^o-r^p)^{2}e^{ \sigma^{r,o}}
-
\sum_{m=1}^{M_{l}}\frac{1}{2}(r_{lm}-r_{l}^o)^{2}e^{ \tau_{l}^r }
+C
} 
\end{align*}



\begin{center}
\line(1,0){250}
\end{center}

\begin{align*}
y_{lmn} &\sim \operatorname{N}(\hat{y}_{lmn},(e^{ \nu_{l}  })^{-1} ) \\
\hat{y}_{lmn} &= f(x_{lmn};e^{ K_{lm} } ,e^{ r_{lm} } , e^{ P })\\
\nu_{l} &\sim \operatorname{N}(\nu^p, (e^{ {\sigma}^{\nu} })^{-1} )\\
\\
\pi(\nu_{l}|\theta)&=
\sqrt{\frac{e^{ {\sigma}^{\nu} }}{2\pi}} e^{-\frac{1}{2}(\nu_{l}-\nu^p)^{2}e^{ {\sigma}^{\nu} }}
\prod_{m=1}^{m_{l}}\prod_{n=1}^{n_{lm}}
\sqrt{\frac{e^{ \nu_{l}}}{2\pi}} e^{-\frac{1}{2}(y_{lmn}-\hat{y}_{lmn})^{2}e^{ \nu_{l}} }\\
\text{Taking logs}\\
\color{red}{l\pi(\nu_{l}|\theta)}&
\color{red}{
=-\frac{1}{2}(\nu_{l}-\nu^p)^{2}e^{ {\sigma}^{\nu}}
+
\sum_{m=1}^{m_{l}}\sum_{n=1}^{n_{lm}}\frac{1}{2}(\nu_{l}-(y_{lmn}-\hat{y}_{lmn})^{2}e^{\nu_{l}})
+C
}
\end{align*}

\begin{center}
\line(1,0){250}
\end{center}

\begin{align*}
K_{l}^o &\sim \operatorname{N}(K^p, (e^{ \sigma^{K,o} })^{-1} )\\
\sigma^{K,o} &\sim \operatorname{N}(\eta^{K,o}, (\psi^{K,o})^{-1} )\\
\pi(\sigma^{K,o}|\theta)&=
\sqrt{\frac{\psi^{K,o}}{2\pi}} e^{-\frac{1}{2}(\sigma^{K,o}-\eta^{K,o})^{2}\psi^{K,o} }
\prod_{l=1}^{L}
\sqrt{\frac{e^{ \sigma^{K,o} }}{2\pi}} e^{-\frac{1}{2}(K_{l}^o-K^p)^{2} e^{ \sigma^{K,o} }}\\
\text{Taking logs}\\
\color{red}{l\pi(\sigma^{K,o}|\theta)}&
\color{red}{
=-\frac{1}{2}(\sigma^{K,o}-\eta^{K,o})^{2}\psi^{K,o}
+
\sum_{l=1}^{L}\frac{1}{2}(\sigma^{K,o} -(K_{l}^o-K^p)^{2}e^{ \sigma^{K,o} })
+C
}\\
\text{Similarly for $\sigma^{r,o}$}\\
\color{red}{l\pi(\sigma^{r,o}|\theta)}&
\color{red}{
=-\frac{1}{2}(\sigma^{r,o}-\eta^{r,o})^{2}\psi^{r,o}
+
\sum_{l=1}^{L}\frac{1}{2}(\sigma^{r,o} -(r_{l}^o-r^p)^{2}e^{ \sigma^{r,o} })
+C
}\\
\text{And also for $\sigma^{\nu}$}\\
\color{red}{l\pi(\sigma^{\nu}|\theta)}&
\color{red}{
=-\frac{1}{2}(\sigma^{\nu}-\eta^{\nu})^{2}\psi^{\nu}
+
\sum_{l=1}^{L}\frac{1}{2}(\sigma^{\nu} -(\nu_{l}-\nu^p)^{2}e^{ \sigma^{\nu} })
+C
}
\end{align*}